\[
\begin{prooftree}
\hypo{
	\langle a, \sigma \rangle \rightarrow
	\langle a^\prime, \sigma \rangle 
} 
\infer1{
	\langle x = a, \sigma \rangle \rightarrow  
	\langle x = a^\prime, \sigma \rangle
}
\end{prooftree} \; \; \; [\text{Assign-A}]
\]


\[
\begin{prooftree}
\infer0{
	\langle x = n, \sigma \rangle \rightarrow  
	\langle \textbf{skip},  \sigma[x \mapsto n] \rangle
}
\end{prooftree} \; \; \; [\text{Assign-N}]
\]

\[
\begin{prooftree}
\hypo{
	\langle c_0, \sigma \rangle \rightarrow
	\langle c_0^\prime, \sigma^\prime \rangle 
} 
\infer1{
	\langle c_0; c_1,  \sigma \rangle \rightarrow  
	\langle c_0^\prime; c_1, \sigma^\prime \rangle
}
\end{prooftree} \; \; \; [\text{Sequence-A}]
\]

\[
\begin{prooftree}
\infer0{
	\langle \textbf{skip}; c_1,  \sigma \rangle \rightarrow  
	\langle c_1, \sigma \rangle
}
\end{prooftree} \; \; \; [\text{Sequence-Skip}]
\]

\[
\begin{prooftree}
\hypo{
	\langle b, \sigma \rangle \rightarrow
	\langle b^\prime, \sigma \rangle 
} 
\infer1{
	\langle \textbf{if } b \textbf{ then } c_0 \textbf{ else } c_1, \sigma   \rangle
	\rightarrow
	\langle \textbf{if } b^\prime \textbf{ then } c_0 \textbf{ else } c_1, \sigma  \rangle
}
\end{prooftree} \; \; \; [\text{Conditional}]
\]

\[
\begin{prooftree}
\infer0{
\langle \textbf{if } \textbf{true} \textbf{ then } c_0 \textbf{ else } c_1, \sigma  \rangle
\rightarrow
\langle c_0, \sigma \rangle 
}
\end{prooftree} \; \; \; [\text{Conditional-True}]
\]

\[
\begin{prooftree}
\infer0{
\langle \textbf{if } \textbf{false} \textbf{ then } c_0 \textbf{ else } c_1, \sigma  \rangle
\rightarrow
\langle c_1, \sigma \rangle 
}
\end{prooftree} \; \; \; [\text{Conditional-False}]
\]

\[
\begin{prooftree}
\infer0{
\langle \textbf{while } b \textbf{ do } c, \sigma \rangle
\rightarrow
\langle \textbf{if } b \textbf{ then } (c; \textbf{while } b \textbf{ do } c)
\textbf{ else } \textbf{skip}, \sigma \rangle
}
\end{prooftree} \; \; \; [\text{While}]
\]
