\[
\begin{prooftree}
\infer0{
	\langle x, \sigma \rangle 
	\rightarrow  
	\langle \sigma(x), \sigma \rangle 
}
\end{prooftree} \; \; \; [\text{Variable}]
\]

\[
\begin{prooftree}
\hypo{
	\langle a_1, \sigma \rangle \rightarrow
	\langle a_1^\prime, \sigma \rangle 
} 
\infer1{
	\langle a_1 \oplus a_2, \sigma \rangle \rightarrow  
	\langle a_1^\prime \oplus a_2, \sigma \rangle
}
\end{prooftree} \; \oplus = \{+,\times\} \; \; \; [\text{AExp-Lhs-}\oplus]
\]

\[
\begin{prooftree}
\hypo{
	\langle a_2, \sigma \rangle \rightarrow
	\langle a_2^\prime, \sigma \rangle 
} 
\infer1{
	\langle a_1 \oplus a_2, \sigma \rangle \rightarrow  
	\langle a_1 \oplus a_2^\prime, \sigma \rangle
}
\end{prooftree} \; \oplus = \{+,\times\} \; \; \; [\text{AExp-Rhs-}\oplus]
\]

\[
\begin{prooftree}
\infer0{
	\langle n_1 \oplus n_2, \sigma \rangle \rightarrow  
	\langle n_3,  \sigma \rangle
}
\end{prooftree} \; \; \; \; \oplus = \{+,\times\}, n_3 \in \mathbb{Z} \; \; \; [\text{AExp-}\oplus]
\]

