\section{RedexMatchAssertEqual Form}
Given \RedexMatchAssertEqual, code generation proceeds in the following manner.

\begin{enumerate}
\item First, generate a list of expected matches \texttt{expectedmatches}. For each $m_i =$ \Match,
\begin{enumerate}
\item Generate the function $f_{t_i}$ for $t_i$ and let resulting the term be $tt_i = f_{t_i}(Match())$
\item Create an empty \texttt{Match} instance \texttt{match}, call \texttt{match.AddBinding}$(s_i)$ and \newline \texttt{match.AddToBinding}$(tt_i)$ methods, and then append \texttt{match} to \texttt{matches}.
\end{enumerate}
\item Generate the top-level matching function $f_p^{top}$ for pattern $p$ and the term-generating function $f_t$ for term-template $t$.
\item Let \texttt{actualmatches} = $f_p(f_t(Match()))$ and then call \texttt{assert\_compare\_match\_lists} with \texttt{expectedmatches} and \texttt{actualmatches}.
\end{enumerate}

\begin{figure}[h]
\begin{minted}[tabsize=2,obeytabs,escapeinside=||,mathescape=true,fontsize=\normalsize]{python}
{% def codegenRedexMatchAssertEqual(|$rm$|): %}
	{% |$f_{rm}$| = symgen("redexmatchassertequal") %}
		{% |$f_p^{top}$| = codegenTopLevelPattern(|$rm$|[|$p$|]) %}
			{% |$f_t$| = codegenTermTemplate(|$rm$|[|$t$|]) %}
def |$f_{rm}$|():
	{% for |$m_i$| in |$rm$|[|$m_1, ..., m_n$|]: %}
	|$mi_i$| = Match()
		{% for |$(s_i, t_i)$| in |$m_i$[$(s_1, t_1), ..., (s_m, t_m)$]|: %}
			{% |$f_{t_i}$| = CodegenTermTemplate(|$t_i$|) %}
	term = |$f_{t_i}$|(Match())
	|$mi_i$|.addkey(|$s_i$|)
	|$mi_i$|.addbinding(|$s_i$|, term)
		{% endfor %}
	{% endfor %}
	expectedmatches = [|$mi_1, ..., mi_n$|]
	term = |$f_t$|(Match())
	actualmatches = |$f_p^{top}$|(term)
	assert_compare_match_lists(actualmatches, expectedmatches)
{% return |$f_{rm}$| %}
{% enddef %}
\end{minted}
\caption{Code generation for \RedexMatchAssertEqualNoArgs \space form.}
\label{codegen-redexmatch}
\end{figure}

\section{TermLetAssertEqual Form}

Given $tl=$ \TermLetAssertEqual, code generation proceeds in the following manner.
\begin{enumerate}
	\item First, produce the \texttt{Match} instance containing all pattern-variable $v_i$ assignments. Let $m=$ \texttt{Match()}. For each $(v_i, n_i, t_i)$
	\begin{enumerate}
	\item Generate the $f_{t_i}$ function for term $t_i$.
	\item $m$.\texttt{AddBinding}$(v_i)$ and $m$.\texttt{AddToBinding}$(v_i, f_{t_i}(\texttt{Match()}))$
	\end{enumerate}
\item Generate $f_t$ for term-template $t$ and $f_e$ for the term-template $e$.
\item Call \texttt{asserttermsequal}$(f_t(m), f_e(\texttt{\texttt{Match()}}))$.
\end{enumerate}

\begin{figure}[htb]
\begin{minted}[tabsize=2,obeytabs,escapeinside=||,mathescape=true,fontsize=\normalsize]{python}
{% def codegenTermLetAssertEqual(|$tl$|): %}
	{% |$f_{tl}$| = symgen("termletassertequal") %}
	{% |$f_t$| = codegenTermTemplate(|$tl$|[|$t$|]) %}
	{% |$f_e$| = codegenTermTemplate(|$tl$|[|$e$|]) %}
def |$f_{tl}$|():
	match = Match()
	{% for |$(v_i, n_i, t_i)$| in |$tl$|[|$(v_1, n_1, t_1)$|, ..., |$(v_n, n_n, t_n)$|]: %}
		{% |$f_{t_i}$| = codegenTermTemplate(|$t_i$|) %}
	term = |$f_{t_i}$|(Match())
	match.addkey(|$v_i$|)
	match.addtobinding(|$v_i$|, term)
	{% endfor %}
	expected = |$f_e$|(Match())
	actual = |$f_t$|(match)
	asserttermsequal(expected, actual)
{% return |$f_{tl}$|  %}
{% enddef %}
\end{minted}
\caption{Code generation for \TermLetAssertEqualNoArgs \space form.}
\label{codegen-termlet}
\end{figure}


\section{ApplyReductionRelationAssertEqual Form}

Given \ApplyReductionRelationAssertEqual:
\begin{enumerate}
\item First, generate a list of expected terms \texttt{expected}, potentially empty.
	\begin{enumerate}
	\item Generate the function $f_{e_i}$ for each term-template $e_i$.
	\item Concatenate the results of $f_{e_i}(\texttt{Match()})$ to \texttt{expected}.
	\end{enumerate}
\item Generate the function $f_t$ for the term-template $t$.
\item Let $f_{red}$ be a Python function for \DefineReductionRelationNoArgs \space with the name $r$. Let \texttt{actual} = $f_{red}(f_t(\texttt{Match()}))$ be the list of terms after applying the reduction relation.
\item Call \texttt{asserttermlistsequal(expected, actual)}.
\end{enumerate}

\begin{figure}[htb]
\begin{minted}[tabsize=2,obeytabs,escapeinside=||,mathescape=true,fontsize=\normalsize]{python}
{% def codegenApplyReductionRelationAssertEqual(|$tl$|): %}
	{% |$f_{tl}$| = symgen("applyreductionrelationassertequal") %}
	{% |$f_{red}$| = get_reduction_relation(|$tl$|[|$r$|]) %}
	{% |$f_t$| = codegenTermTemplate(|$tl$|[|$t$|]) %}
	{% |$f_{e_1}, ..., f_{e_n}$| = codegenTermTemplates(|$tl$|[|$e_1, ..., e_n $|]) %}
def |$f_{ar}$|():
	expected = [|$f_{e_1}(\texttt{Match()}), ..., f_{e_n}(\texttt{Match()})$|]
	actual = |$f_t$|(Match())
	asserttermlistsequal(expected, actual)
{% return |$f_{ar}$| %}
{% enddef %}
\end{minted}
\caption{Code generation for \ApplyReductionRelationAssertEqualNoArgs \space form.}
\label{codegen-applyred}
\end{figure}
